End of day 25/05/18

michael_formal/EFSM.thy
@@ -1,6 +1,14 @@
 theory EFSM
-  imports Constraints
+  imports Types
 begin
+
+primrec apply_outputs :: "output_function list \<Rightarrow> state \<Rightarrow> registers \<Rightarrow> outputs" where
+  "apply_outputs [] _ _ = []" |
+  "apply_outputs (h#t) i r = (aval h (join i r))#(apply_outputs t i r)"
+
+primrec apply_guards :: "guard list \<Rightarrow> state \<Rightarrow> registers \<Rightarrow> bool" where
+  "apply_guards [] _ _ = True" |
+  "apply_guards (h#t) i r =  ((gval h (join i r)) \<and> (apply_guards t i r))"
 
 primrec apply_updates :: "(string \<times> aexp) list \<Rightarrow> state \<Rightarrow> registers \<Rightarrow> registers" where
   "apply_updates [] _ _ = <>" |
@@ -15,7 +23,6 @@ abbreviation possible_steps :: "efsm \<Rightarrow> statename \<Rightarrow> regis
 definition step :: "efsm \<Rightarrow> statename \<Rightarrow> registers \<Rightarrow> label \<Rightarrow> inputs \<Rightarrow> (statename \<times> outputs \<times> registers) option" where
 "step e s r l i \<equiv>
   case (possible_steps e s r l i) of
-    [] \<Rightarrow> None |
     [(s',t)] \<Rightarrow> Some (s', (apply_outputs (Outputs t) (input2state i 1) r), (apply_updates (Updates t) (input2state i 1) r)) |
     _ \<Rightarrow> None"
 
@@ -23,24 +30,16 @@ primrec observe_trace :: "efsm \<Rightarrow> statename \<Rightarrow> registers \
   "observe_trace _ _ _ [] = []" |
   "observe_trace e s r (h#t) = 
     (case (step e s r (fst h) (snd h)) of
-      None \<Rightarrow> [] |
-      Some (s', outputs, updated) \<Rightarrow> (outputs#(observe_trace e s' updated t))
+      Some (s', outputs, updated) \<Rightarrow> (outputs#(observe_trace e s' updated t)) |
+      _ \<Rightarrow> []
     )"
 
 primrec observe_all :: "efsm \<Rightarrow> statename \<Rightarrow> registers \<Rightarrow> trace \<Rightarrow> (statename \<times> outputs \<times> registers) list" where
   "observe_all _ _ _ [] = []" |
   "observe_all e s r (h#t) = 
     (case (step e s r (fst h) (snd h)) of
-      None \<Rightarrow> [] |
-      (Some (s', outputs, updated)) \<Rightarrow> (((s', outputs, updated)#(observe_all e s' updated t)))
-    )"
-
-primrec observe_registers :: "efsm \<Rightarrow> statename \<Rightarrow> registers \<Rightarrow> trace \<Rightarrow> state" where
-  "observe_registers _ _ r [] = r" |
-  "observe_registers e s r (h#t) = 
-    (case (step e s r (fst h) (snd h)) of
-      None \<Rightarrow> r |
-      Some (s', outputs, updated) \<Rightarrow> (observe_registers e s' updated t)
+      (Some (s', outputs, updated)) \<Rightarrow> (((s', outputs, updated)#(observe_all e s' updated t))) |
+      _ \<Rightarrow> []
     )"
 
 definition equiv :: "efsm \<Rightarrow> efsm \<Rightarrow> trace \<Rightarrow> bool" where
@@ -56,11 +55,33 @@ lemma equiv_trans: "equiv e1 e2 t \<and> equiv e2 e3 t \<longrightarrow> equiv e
 lemma equiv_idem: "equiv e1 e1 t"
   by (simp add: equiv_def)
 
-definition valid_trace :: "efsm \<Rightarrow> trace \<Rightarrow> bool" where
-  "valid_trace e t = (length t = length (observe_all e (s0 e) <> t))"
+primrec valid_trace_1 :: "efsm \<Rightarrow> statename \<Rightarrow> registers \<Rightarrow> trace \<Rightarrow> bool" where
+  "valid_trace_1 _ _ _ [] = True" |
+  "valid_trace_1 e s r (h#t) = 
+    (case (step e s r (fst h) (snd h)) of
+      Some (s', _, updated) \<Rightarrow> (valid_trace_1 e s' updated t) |
+      _ \<Rightarrow> False
+    )"
+
+abbreviation valid_trace :: "efsm \<Rightarrow> trace \<Rightarrow> bool" where
+  "valid_trace e t \<equiv> (length t = length (observe_all e (s0 e) <> t))"
+
+lemma "valid_trace e t = valid_trace_1 e (s0 e) <> t"
+proof (induct t)
+  case Nil
+  then show ?case by simp
+next
+  case (Cons a t)
+  then show ?case
+    apply (cases "step e (s0 e) <> (fst a) (snd a)")
+     apply simp
+    apply simp
+    apply safe
+qed
+
 
 lemma empty_trace_valid [simp]: "valid_trace e []"
-  by(simp add:valid_trace_def)
+  by simp
 
 primrec in_list :: "'a \<Rightarrow> 'a list \<Rightarrow> bool" where
   "in_list _ [] = False" |
@@ -75,19 +96,4 @@ definition can_take :: "transition \<Rightarrow> transition \<Rightarrow> bool" 
 primrec find_match :: "transition \<Rightarrow> destination list \<Rightarrow> destination option" where
   "find_match _ [] = None" |
   "find_match t (h#tail) = (if (can_take t (snd h)) then (Some h) else (find_match t tail))"
-
-(*fun match_all :: "efsm \<Rightarrow> destination list \<Rightarrow> efsm \<Rightarrow> destination list \<Rightarrow> statename list \<Rightarrow> bool"
-  and compare :: "efsm \<Rightarrow> statename \<Rightarrow> efsm \<Rightarrow> statename \<Rightarrow> statename list \<Rightarrow> bool"
-  where
-  "match_all _  []    _  _  _      = True" |
-  "match_all e1 (h#t) e2 d2 open = (
-    case (find_match (snd h) d2) of
-      None \<Rightarrow> False |
-      Some (s', _) \<Rightarrow> ((compare e1 (fst h) e2 s' open) \<and> (match_all e1 t e2 d2 open))
-    )" |
-  "compare e1 s1 e2 s2 open = (if (in_list s1 open) then (match_all e1 (all_outs e1 s1) e2 (all_outs e2 s2) (removeAll s1 open)) else True)"
-
-definition simulates :: "efsm \<Rightarrow> efsm \<Rightarrow> bool" where
-  "simulates e1 e2 = compare e1 (s0 e1) e2 (s0 e2) (S e1)"
-*)
 end
