michael_formal/valid_aux.thy
@@ -3,18 +3,17 @@ theory valid_aux
 begin
 
 lemma valid_trace_head_not_none:  "valid_trace efsm [a] \<Longrightarrow> ( step efsm (s0 efsm) <> (fst a) (snd a) \<noteq> None)"
-  apply(simp add:valid_trace_def)
+  apply simp
   apply(cases  "(step efsm (s0 efsm) <> (fst a) (snd a)) = None")
   by(simp_all)
 
 lemma valid_trace_cons: "valid_trace efsm (a#t) \<Longrightarrow> valid_trace efsm [a]"
-  apply(unfold valid_trace_def)
   apply(simp)
   apply(cases  "(step efsm (s0 efsm) <> (fst a) (snd a)) = None")
   apply(simp)
   by auto
 
-lemma lengh_observe_all_restricted: "\<And>s r. length (observe_all e s r t) \<le> length t"
+lemma length_observe_all_restricted: "\<And>s r. length (observe_all e s r t) \<le> length t"
 proof (induction t) 
   case Nil
   then show ?case by simp
@@ -29,6 +28,72 @@ next
     with Cons show ?thesis by(auto) 
   qed
 qed
+
+abbreviation "reg_of t \<equiv> (if t = [] then <> else snd (snd (last t)))"
+abbreviation "state_of e t \<equiv> (if t = [] then s0 e else fst (last t))"
+
+(* abbreviation "drop_last a \<equiv> rev (tl (rev a))" *)
+
+function drop_last :: "'a list \<Rightarrow> 'a list" where
+"drop_last [] = []" |
+"drop_last (xs@[x]) = xs"
+  using rev_exhaust apply blast
+  by simp_all
+termination drop_last
+  using "termination" by blast
+
+function last :: "'a list \<Rightarrow> 'a list" where
+"last [] = []" |
+"last (xs@[x]) = [x]"
+  using rev_exhaust apply blast
+  by simp_all
+termination last
+  using "termination" by blast
+
+lemma foo: "step e (s0 e) <> (fst a) (snd a) = None \<or>  (\<exists>s' outputs updated. step e (s0 e) <> (fst a) (snd a) = Some (s', outputs, updated))"
+  apply (cases "step e (s0 e) <> (fst a) (snd a)")
+   apply simp
+  by auto
+
+lemma "(valid_trace_1 e (s0 e) <> (ts@[t]) \<longrightarrow> valid_trace_1 e (s0 e) <> ts)" 
+proof (induct ts)
+  case Nil
+  then show ?case by simp
+next
+  case (Cons a ts)
+  then show ?case 
+    apply simp
+    apply (case_tac "step e (s0 e) <> (fst a) (snd a) = None")
+     apply simp
+    apply simp
+
+     
+
+qed
+
+
+  
+
+
+  
+
+lemma "valid_trace e t \<Longrightarrow> ((observe_all e (s0 e) <> (drop_last t)) = xs \<longrightarrow> (observe_all e (s0 e) <> t) = xs@(observe_all e (state_of e xs) (reg_of xs) (last t)))"
+proof (induct t rule: rev_induct)
+  case Nil
+  then show ?case by simp
+next
+  case (snoc y ys)
+  then show ?case 
+    apply simp
+     apply (case_tac "step e (s0 e) <> (fst y) (snd y) = None")
+      apply simp
+
+qed
+
+
+  
+
+
 
 
 end
