michael_formal/Constraints.thy
@@ -1,5 +1,5 @@
 theory Constraints
-imports Types CExp
+imports Types EFSM CExp
 
 begin
 
@@ -133,14 +133,6 @@ lemma "subsumes (\<lambda>x. Bc True) (\<lambda>x. Bc False)"
 
 lemma subsumes_reflexivity:  "subsumes x x"
   by (simp add: subsumes_def)
-
-primrec apply_outputs :: "output_function list \<Rightarrow> state \<Rightarrow> registers \<Rightarrow> outputs" where
-  "apply_outputs [] _ _ = []" |
-  "apply_outputs (h#t) i r = (aval h (join i r))#(apply_outputs t i r)"
-
-primrec apply_guards :: "guard list \<Rightarrow> state \<Rightarrow> registers \<Rightarrow> bool" where
-  "apply_guards [] _ _ = True" |
-  "apply_guards (h#t) i r =  ((gval h (join i r)) \<and> (apply_guards t i r))"
 
 (* Widening the precondition and reducing nondeterminism *)
 (* Guards of A imply guards of B and if the precondition of A is satisfied and we do a B then the
